Modify the Hoare judgment such that is also ensures thread safity.
Before, it just ensured that whenever one can split up the memory
into two parts before running the program, the framing part can
be split off when the program is finished. Now it also ensure that
it can be split off at any moment during the execution of the
program.

When we extend to non-deterministic expressions/sequence points we
certainly need this for the Hoare judgment for expressions, as C
allows evaluation of them to interleave. However, for consistency,
and further extensions, it is nice to have this property for
statements too.

axiomatic.v
@@ -5,11 +5,11 @@ Local Open Scope nat_scope.
 
 Definition dassert := direction → assert.
 Definition dassert_pack (Ψ : (label → assert) * (option N → assert)) 
-    (P : assert) (Q: assert) : direction → assert := 
+    (P : assert) (Q: assert) : direction → assert :=
   direction_rect (λ _, assert) P Q (snd Ψ) (fst Ψ).
 
 Instance: Proper 
-  (prod_relation (pointwise_relation _ (≡)) (pointwise_relation _ (≡)) ==> 
+  (prod_relation (pointwise_relation _ (≡)) (pointwise_relation _ (≡)) ==>
     (≡) ==> (≡) ==> (=) ==> (≡)) dassert_pack.
 Proof. intros ?????????? d ?. subst. destruct d; firstorder. Qed.
 
@@ -18,13 +18,63 @@ Definition dassert_map (f : assert → assert) (P : dassert) : dassert :=
 Lemma dassert_map_spec f P d : dassert_map f P d = f (P d).
 Proof. now destruct d. Qed.
 
-Definition ax (s : stmt) (P : direction → assert) := ∀ A d k m d' k' s' m',
-    State d k s m ⇨{k}* State d' k' s' m' →
-    nf (⇨{k}) (State d' k' s' m') →
+Inductive ax_conclusion (P : dassert) (k : ctx) (mr : mem) (S : state) : Prop :=
+  | ax_further ml :
+     mem_disjoint ml mr →
+     SMem S = ml ∪ mr →
+     red (⇨{k}) S →
+     ax_conclusion P k mr S
+  | ax_done ml :
+     mem_disjoint ml mr →
+     SMem S = ml ∪ mr →
+     SCtx S = k →
+     up (SDir S) (SStmt S) →
+     P (SDir S) (get_stack k) ml →
+     ax_conclusion P k mr S.
+
+Definition ax (s : stmt) (P : dassert) := ∀ d k ml mr S',
+    mem_disjoint ml mr →
+    State d k s (ml ∪ mr) ⇨{k}* S' →
     down d s →
-    (A * P d)%A (get_stack k) m →
-  k' = k ∧ up d' s' ∧ (A * P d')%A (get_stack k) m'.
+    P d (get_stack k) ml →
+  ax_conclusion P k mr S'.
 Notation "Ψ ⊢ ⦃ P ⦄ s ⦃ Q ⦄" := (ax s%S (dassert_pack Ψ%A P%A Q%A)) (at level 80).
+
+Lemma ax_split s P (Hax : ax s P) l n d k ml mr S'' :
+    mem_disjoint ml mr →
+    State d (l ++ k) s (ml ∪ mr) ⇨{k}^n S'' →
+    down d s →
+    P d (get_stack l ++ get_stack k) ml →
+  (∃ ml'',
+    mem_disjoint ml'' mr
+    ∧ SMem S'' = ml'' ∪ mr
+    ∧ red (⇨{l ++ k}) S'')
+  ∨ (∃ n' d' ml',
+    mem_disjoint ml' mr
+    ∧ State d' (l ++ k) s (ml' ∪ mr) ⇨{k}^n' S''
+    ∧ n' ≤ n
+    ∧ up d' s ∧ P d' (get_stack l ++ get_stack k) ml').
+Proof.
+  intros ? p1 Hdown HP.
+  rewrite <-get_stack_app in *.
+  destruct (cstep_subctx_cut l k _ _ _ p1)
+    as [? | [n' [S' [p2 [p3 [??]]]]]]; eauto with list.
+   destruct (Hax d (l ++ k) ml mr S'') as [ml'' | ml'']; auto.
+    left. exists ml''. now auto.
+   destruct S'' as [d'' k'' s'' m'']; simpl in *.
+   right. exists 0 d'' ml''.
+   assert (s = s''); subst.
+    eapply csteps_preserve_stmt.
+    now apply (rtc_subrel (⇨{l ++ k}) (⇨) _); eauto.
+   now intuition.
+  right. destruct (Hax d (l ++ k) ml mr S') as [ml' | ml']; auto.
+   exists n' (SDir S') ml'. now auto.
+  destruct S' as [d' k' s' m']; simpl in *.
+  assert (s = s'); subst.
+   eapply csteps_preserve_stmt.
+   now apply (rtc_subrel (⇨{l ++ k}) (⇨) _); eauto.
+  exists n' d' ml'. now auto.
+Qed.
 
 Lemma ax_sound s P d m d' k' s' m' :
   ax s P →
@@ -37,175 +87,175 @@ Lemma ax_sound s P d m d' k' s' m' :
   ∧ P d' [] m'.
 Proof.
   intros Hax p Hnf ??.
-  destruct (Hax emp%A d [] m d' k' s' m') as [? [??]].
-      now apply (rtc_subrel (⇨) (⇨{[]}) _).
-     now apply (nf_subrel (⇨{[]}) (⇨) _).
-    easy.
-   now apply assert_sep_left_id_2.
-  intuition. now apply assert_sep_left_id_1.
+  destruct (Hax d [] m ∅ (State d' k' s' m')) as [m'' | m'']; auto.
+  * auto with mem.
+  * rewrite (right_id ∅ _). now apply (rtc_subrel (⇨) (⇨{[]}) _).
+  * destruct Hnf. now apply (red_subrel (⇨{[]}) _ _).
+  * simpl in *. subst. rewrite (right_id ∅ _). now auto.
 Qed.
 
 Lemma ax_weak Ψ P Q s : 
   Ψ ⊢ ⦃ P ⦄ s ⦃ Q ⦄ → ∀ P' Q', P' ⊆ P → Q ⊆ Q' → Ψ ⊢ ⦃ P' ⦄ s ⦃ Q' ⦄.
 Proof.
-  intros Hax P' Q' HP HQ A d k m d' k' s' m' ????.
-  destruct (Hax A d k m d' k' s' m'); auto.
-   destruct d; simpl in *; intuition. now rewrite <-HP.
-  destruct d'; simpl in *; intuition. now rewrite <-HQ.
+  intros Hax P' Q' HP HQ d k ml mr S' ????.
+  destruct (Hax d k ml mr S') as [ml' | ml']; auto.
+    now destruct d; intuition.
+   now left with ml'.
+  right with ml'; auto. destruct (SDir S'); intuition.
+Qed.
+
+Lemma ax_frame_packed A Ppack s :
+  ax s Ppack → ax s (dassert_map (λ P, P * A)%A Ppack).
+Proof.
+  intros Hax d k m1 m4 S' ???.
+  rewrite dassert_map_spec.
+  intros [m2 [m3 [? [? [??]]]]]. subst.
+  destruct (Hax d k m2 (m3 ∪ m4) S') as [ml2' | ml2']; auto.
+     solve_mem_disjoint.
+    now rewrite (associative _).
+   left with (ml2' ∪ m3); auto.
+    solve_mem_disjoint.
+   now rewrite <-(associative _).
+  right with (ml2' ∪ m3); auto.
+    solve_mem_disjoint.
+   now rewrite <-(associative _).
+  rewrite dassert_map_spec.
+  exists ml2' m3. intuition. solve_mem_disjoint.
 Qed.
 
 Lemma ax_frame J R A P Q s :
-  (J,R) ⊢ ⦃ P ⦄ s ⦃ Q ⦄ → (λ l, A * J l, λ v, A * R v) ⊢ ⦃ A * P ⦄ s ⦃ A * Q ⦄.
-Proof.
-  intros Hax B d k m d' k' s' m' ????.
-  destruct (Hax (B * A)%A d k m d' k' s' m'); auto.
-   destruct d; simpl in *; intuition; now rewrite <-(associative _).
-  destruct d'; simpl in *; intuition; now rewrite (associative _).
-Qed.
+  (J,R) ⊢ ⦃ P ⦄ s ⦃ Q ⦄ → (λ l, J l * A, λ v, R v * A) ⊢ ⦃ P * A ⦄ s ⦃ Q * A ⦄.
+Proof. apply ax_frame_packed. Qed.
 
 Lemma ax_and Ψ P Q Q' s :
   Ψ ⊢ ⦃ P ⦄ s ⦃ Q ⦄ → Ψ ⊢ ⦃ P ⦄ s ⦃ Q' ⦄ → Ψ ⊢ ⦃ P ⦄ s ⦃ Q ∧ Q' ⦄.
 Proof.
-  intros Hax Hax' B d k m d' k' s' m' ??? Hpre.
-  destruct Hpre as [m1 [m2 [? [? [??]]]]].
-  (* The Separation judgment does not directly say that the splitting of the
-   memory before and after are the same. However, by extending the frame
-   condition with an equality on the memory we do get that result *)
-  destruct (Hax (Assert $ λ ρ m, m = m1 ∧ B ρ m) d k m d' k' s' m')
-     as [? [? [m1' [m2' [? [? [[??] ?]]]]]]]; auto.
-   exists m1 m2; destruct d; intuition.
-  destruct (Hax' (Assert $ λ ρ m, m = m1 ∧ B ρ m) d k m d' k' s' m')
-     as [_ [_ [m1'' [m2'' [? [? [[??] ?]]]]]]]; auto.
-   exists m1 m2; destruct d; intuition.
-  assert (m2'' = m2'); subst.
-   apply mem_union_cancel_r with m1; auto; now symmetry.
-  intuition. exists m1 m2'. intuition.
-  destruct d'; intuition. now split.
+  intros Hax1 Hax2 d k ml mr S' ??? Hpre.
+  destruct (Hax1 d k ml mr S') as [ml' | ml']; auto.
+    now destruct d; intuition.
+   now left with ml'.
+  destruct (Hax2 d k ml mr S') as [ml'' | ml'']; auto.
+    now destruct d; intuition.
+   now left with ml'.
+  assert (ml' = ml''); subst.
+   now apply mem_union_cancel_l with mr; intuition congruence.
+  right with ml''; auto.
+  destruct (SDir S'); intuition auto. now split.
 Qed.
 
 Lemma ax_skip Ψ P : Ψ ⊢ ⦃ P ⦄ skip ⦃ P ⦄.
 Proof.
-  intros A d k m d' k' s' m' p ???. inv_csteps p as [ | ???? p].
-   solve_cnf.
-  inv_cstep. inv_csteps p.
-   intuition.
+  intros d k ml mr S' ? p ??. inv_csteps p as [ | ???? p].
+   left with ml; auto. solve_cnf.
+  inv_cstep. inv_csteps p; simpl in *.
+   now right with ml.
   inv_cstep.
 Qed.
 
 Lemma ax_goto Ψ Q l : Ψ ⊢ ⦃ fst Ψ l ⦄ goto l ⦃ Q ⦄.
 Proof.
-  intros A d k m d' k' s' m' p ???. inv_csteps p as [ |???? p].
-   solve_cnf.
-  inv_cstep. inv_csteps p.
-   intuition simplify_elem_of.
+  intros d k ml mr S' ? p ??. inv_csteps p as [ | ???? p].
+   left with ml; auto. solve_cnf.
+  inv_cstep. inv_csteps p; simpl in *.
+   right with ml; auto. simplify_elem_of.
   inv_cstep.
 Qed.
 
 Lemma ax_return Ψ e Q : Ψ ⊢ ⦃ ∃ v, e⇓v ∧ snd Ψ (Some v) ⦄ ret e ⦃ Q ⦄.
 Proof.
-  intros A d k m d' k' s' m' p ?? Hpre.
+  intros d k ml mr S' ? p ? Hpre.
   destruct d; try contradiction.
-  destruct Hpre as [m1 [m2 [? [? [? [v [??]]]]]]]; subst.
-  inv_csteps p as [| ???? p ].
-   simplify_assert_expr. solve_cnf.
-  inv_cstep. inv_csteps p.
-   intuition eauto. simplify_assert_expr. solve_assert.
+  destruct Hpre as [v [??]]. simplify_assert_expr.
+  inv_csteps p as [| ???? p ]; simpl in *.
+   left with ml; auto. solve_cnf.
+  inv_cstep. inv_csteps p; simpl in *.
+   simplify_assert_expr.
+   now right with ml.
   inv_cstep.
 Qed.
 
 Lemma ax_assign Ψ e1 e2 (Q : assert) :
   Ψ ⊢ ⦃ ∃ a v, e1⇓a ∧ e2⇓v ∧ load a⇓- ∧ <[a:=v]>Q ⦄ e1 ::= e2 ⦃ Q ⦄.
 Proof.
-  intros A d k m d' k' s' m' p ?? Hpre.
+  intros d k ml mr S' ? p ? Hpre.
   destruct d; try contradiction.
-  inv_csteps p as [| ???? p ].
-   destruct Hpre as [m1 [m2 [? [? [? [a [v [? [? [[??] ?]]]]]]]]]]; subst.
-   assert (is_writable a (m1 ∪ m2)).
-     do 2 red. eauto with mem.
-   simplify_assert_expr. solve_cnf.
-  inv_cstep. inv_csteps p.
-   intuition. simpl in *. eapply assert_assign; eauto.
+  inv_csteps p as [| ???? p ]; simpl in *.
+   left with ml; auto.
+   destruct Hpre as [a [v [? [? [[??] ?]]]]].
+   simplify_assert_expr.
+   assert (is_writable a (ml ∪ mr)).
+    do 2 red. eauto with mem.
+   solve_cnf.
+  inv_cstep. inv_csteps p; simpl in *.
+   destruct Hpre as [a' [v' [? [? [[??] ?]]]]].
+   simplify_assert_expr.
+   right with (<[a:=v]>ml); auto.
+    now eauto with mem.
+   now rewrite mem_union_insert_l.
   inv_cstep.
-Qed.
-
-Lemma ax_split s P :
-  ax s P → ∀ l n A d k m S',
-    State d (l ++ k) s m ⇨{k}^n S' →
-    nf (⇨{k}) S' →
-    down d s →
-    (A * P d)%A (get_stack l ++ get_stack k) m →
-  ∃ n' d' m',
-    State d' (l ++ k) s m' ⇨{k}^n' S'
-    ∧ up d' s
-    ∧ (A * P d')%A (get_stack l ++ get_stack k) m'
-    ∧ n' ≤ n.
-Proof.
-  intros Hax l n A d k m S' p1 Hnf Hdown HP.
-  rewrite <-get_stack_app in *.
-  destruct (cstep_subctx_cut l k _ _ _ p1) as [n' [[d' k' s' m'] ?]]; eauto with list.
-  destruct (Hax A d (l ++ k) m d' k' s' m'); intuition.
-  assert (s = s'); subst.
-   eapply csteps_preserve_stmt.
-   apply (rtc_subrel (⇨{l ++ k}) (⇨) _); eauto.
-  exists n' d' m'. intuition.
 Qed.
 
 Lemma ax_loop Ψ P Q s : Ψ ⊢ ⦃ P ⦄ s ⦃ P ⦄ → Ψ ⊢ ⦃ P ⦄ loop s ⦃ Q ⦄.
 Proof.
-  intros Hax A d k m d5 k5 s5 m5 p Hnf. revert d m p.
-  assert (∀ n d m,
-    State d (CItem (loop □) :: k) s m ⇨{k}^n State d5 k5 s5 m5 →
-    down d s →
-    (A * dassert_pack Ψ P P d)%A (get_stack k) m →
-      k5 = k ∧ up d5 s5 ∧ (A * dassert_pack Ψ P Q d5)%A (get_stack k) m5
-   ).
-   induction n as [n IH] using lt_wf_ind.
-   intros d1 m1 p1 ??.
-   edestruct (ax_split _ _ Hax [CItem (loop □)])
-     as [n' [d2 [m2 [p2 [? [??]]]]]]; simpl in *; eauto.
-   inv_csteps p2 as [| n'' ? S3 ? p2 p3].
-    solve_cnf.
+  intros Hax d k ml mr S5 Hdisjoint p1.
+  revert d ml Hdisjoint p1.
+  assert (∀ n d ml,
+      mem_disjoint ml mr →
+      State d (CItem (loop □) :: k) s (ml ∪ mr) ⇨{k}^n S5 →
+      down d s →
+      dassert_pack Ψ P P d (get_stack k) ml →
+    ax_conclusion (dassert_pack Ψ P Q) k mr S5).
+   induction n as [n1 IH] using lt_wf_ind.
+   intros d1 ml1 ? p1 ??.
+   edestruct (ax_split s _ Hax [CItem (loop □)])
+     as [[ml2 [? [??]]] | [n' [d2 [ml2 [? [p2 ?]]]]]]; simpl in *; eauto.
+    left with ml2; auto. solve_cnf.
+   inv_csteps p2 as [| n3 ? S3 ? p2 p3]; simpl in *.
+    left with ml2; auto. solve_cnf.
    { inv_cstep p2; try solve [simplify_stmt_elem_of].
-   * inv_csteps p3 as [| n''' ? S4 ? p3 p4].
-       solve_cnf.
-      inv_cstep. eapply (IH n'''); eauto. omega.
-   * inv_csteps p3; eauto. inv_cstep.
-   * inv_csteps p3; eauto. inv_cstep. }
-  intros d m p ??.
-  destruct (rtc_nsteps p) as [n pn]. inv_csteps pn.
-   solve_cnf.
+   * inv_csteps p3 as [| n4 ? S4 ? p3 p4]; simpl in *.
+       left with ml2; auto. solve_cnf.
+      inv_cstep. eapply (IH n4); intuition eauto. omega.
+   * inv_csteps p3; simpl in *. now right with ml2. inv_cstep.
+   * inv_csteps p3; simpl in *. now right with ml2. inv_cstep. }
+  intros d ml ? p ??.
+  destruct (rtc_nsteps p) as [n pn]. inv_csteps pn; simpl in*.
+   left with ml; auto. solve_cnf.
   inv_cstep; eauto.
 Qed.
 
 Lemma ax_label Ψ l s Q :
   Ψ ⊢ ⦃ fst Ψ l ⦄ s ⦃ Q ⦄ → Ψ ⊢ ⦃ fst Ψ l ⦄ l :; s ⦃ Q ⦄.
 Proof.
-  intros Hax A d k m d5 k5 s5 m5 p Hnf. revert d m p.
-  assert (∀ n d m,
-    State d (CItem (l :; □) :: k) s m ⇨{k}^n State d5 k5 s5 m5 →
-    down d s →
-    (A * dassert_pack Ψ (fst Ψ l) Q d)%A (get_stack k) m →
-      k5 = k ∧ up d5 s5 ∧ (A * dassert_pack Ψ (fst Ψ l) Q d5)%A (get_stack k) m5
-   ).
-   induction n as [n IH] using lt_wf_ind.
-   intros d1 m1 p1 ??.
-   edestruct (ax_split _ _ Hax [CItem (l :; □)])
-     as [n' [d2 [m2 [p2 [? [??]]]]]]; simpl in *; eauto.
-   inv_csteps p2 as [| n'' ? S3 ? p2 p3].
-    solve_cnf.
+  intros Hax d k ml mr S5 Hdisjoint p1.
+  revert d ml Hdisjoint p1.
+  assert (∀ n d ml,
+      mem_disjoint ml mr →
+      State d (CItem (l :; □) :: k) s (ml ∪ mr) ⇨{k}^n S5 →
+      down d s →
+      dassert_pack Ψ (fst Ψ l) Q d (get_stack k) ml →
+    ax_conclusion (dassert_pack Ψ (fst Ψ l) Q) k mr S5).
+   induction n as [n1 IH] using lt_wf_ind.
+   intros d1 ml1 ? p1 ??.
+   edestruct (ax_split s _ Hax [CItem (l :; □)])
+     as [[ml2 [? [??]]] | [n' [d2 [ml2 [? [p2 ?]]]]]]; simpl in *; eauto.
+    left with ml2; auto. solve_cnf.
+   inv_csteps p2 as [| n3 ? S3 ? p2 p3]; simpl in *.
+    left with ml2; auto. solve_cnf.
    { inv_cstep p2; try solve [simplify_stmt_elem_of].
-   * inv_csteps p3; eauto. inv_cstep.
-   * inv_csteps p3; eauto. inv_cstep.
+   * inv_csteps p3; simpl in *. now right with ml2. inv_cstep.
+   * inv_csteps p3; simpl in *. now right with ml2. inv_cstep.
    * match goal with
      | _ : State (Goto ?l') _ _ _ ⇨{_}^_ _ |- _ => destruct (decide (l' = l))
      end; simpl in *; subst.
-    + inv_csteps p3 as [| n''' ? S4 ? p3 p4].
-         solve_cnf.
-        inv_cstep. eapply (IH n'''); eauto. omega.
-    + inv_csteps p3. simplify_elem_of. inv_cstep. }
-  intros d m p ??.
-  destruct (rtc_nsteps p) as [n pn]. inv_csteps pn.
-   destruct d5; try contradiction; simpl in *; simplify_elem_of; solve_cnf.
+    + inv_csteps p3 as [| n4 ? S4 ? p3 p4]; simpl in *.
+         left with ml2; auto. solve_cnf.
+        inv_cstep. eapply (IH n4); intuition eauto. omega.
+    + inv_csteps p3; simpl in *. right with ml2; simplify_elem_of. inv_cstep. }
+  intros d ml ? p ??.
+  destruct (rtc_nsteps p) as [n pn]. inv_csteps pn; simpl in *.
+   left with ml; auto.
+   destruct d; simplify_elem_of; solve_cnf. 
   inv_cstep; eauto.
 Qed.
 
@@ -214,49 +264,53 @@ Lemma ax_comp Ψ sl sr P P' Q :
   Ψ ⊢ ⦃ P' ⦄ sr ⦃ Q ⦄ →
   Ψ ⊢ ⦃ P ⦄ sl ;; sr ⦃ Q ⦄.
 Proof.
-  intros Haxl Haxr A d k m d5 k5 s5 m5 p Hnf. revert d m p.
-  assert (∀ n d m,
-    (State d (CItem (□ ;; sr) :: k) sl m ⇨{k}^n State d5 k5 s5 m5 
+  intros Haxl Haxr d k ml mr S5 Hdisjoint p1.
+  revert d ml Hdisjoint p1.
+  assert (∀ n d ml,
+    mem_disjoint ml mr →
+    (State d (CItem (□ ;; sr) :: k) sl (ml ∪ mr) ⇨{k}^n S5
       ∧ down d sl
-      ∧ (A * dassert_pack Ψ P P' d)%A (get_stack k) m)
-    ∨ (State d (CItem (sl ;; □) :: k) sr m ⇨{k}^n State d5 k5 s5 m5
+      ∧ dassert_pack Ψ P P' d (get_stack k) ml)
+    ∨ (State d (CItem (sl ;; □) :: k) sr (ml ∪ mr) ⇨{k}^n S5
       ∧ down d sr
-      ∧ (A * dassert_pack Ψ P' Q d)%A (get_stack k) m) →
-    k5 = k ∧ up d5 s5 ∧ (A * dassert_pack Ψ P Q d5)%A (get_stack k) m5
-   ).
+      ∧ dassert_pack Ψ P' Q d (get_stack k) ml) →
+    ax_conclusion (dassert_pack Ψ P Q) k mr S5).
    induction n as [n IH] using lt_wf_ind.
-   intros d1 m1 [[p1 [??]] | [p1 [??]]].
-    edestruct (ax_split _ _ Haxl [CItem (□ ;; sr)])
-      as [n' [d2 [m2 [p2 [? [??]]]]]]; simpl in *; eauto.
-    inv_csteps p2 as [| n'' ? S3 ? p2 p3].
-     solve_cnf.
+   intros d1 ml1 ? [[p1 [??]] | [p1 [??]]].
+    edestruct (ax_split sl _ Haxl [CItem (□ ;; sr)])
+      as [[ml2 [? [??]]] | [n' [d2 [ml2 [? [p2 ?]]]]]]; simpl in *; eauto.
+     left with ml2; auto. solve_cnf.
+    inv_csteps p2 as [| n3 ? S3 ? p2 p3]; simpl in *.
+     left with ml2; auto. solve_cnf.
     { inv_cstep p2; try solve [simplify_stmt_elem_of].
-    * eapply (IH n''); eauto.
-    * inv_csteps p3; eauto. inv_cstep.
+    * eapply (IH n3); intuition eauto.
+    * inv_csteps p3; simpl in *. now right with ml2. inv_cstep.
     * match goal with
-      | _ : State (Goto ?l') _ _ _ ⇨{_}^_ _ |- _ => destruct (decide (l ∈ labels sr))
-      end; simpl in *; subst.
-     + inv_csteps p3 as [| n''' ? S4 ? p3 p4].
-          solve_cnf.
-         inv_cstep. eapply (IH n'''); eauto. omega.
-     + inv_csteps p3. simplify_elem_of. inv_cstep. }
-   edestruct (ax_split _ _ Haxr [CItem (sl ;; □)])
-     as [n' [d2 [m2 [p2 [? [??]]]]]]; simpl in *; eauto.
-   inv_csteps p2 as [| n'' ? S3 ? p2 p3].
-    solve_cnf.
-   { inv_cstep p2; try solve [simplify_stmt_elem_of].
-   * inv_csteps p3; eauto. inv_cstep.
-   * inv_csteps p3; eauto. inv_cstep.
-   * match goal with
-     | _ : State (Goto ?l') _ _ _ ⇨{_}^_ _ |- _ => destruct (decide (l ∈ labels sl))
+     | _ : State (Goto ?l') _ _ _ ⇨{_}^_ _ |- _ => destruct (decide (l ∈ labels sr))
      end; simpl in *; subst.
-    + inv_csteps p3 as [| n''' ? S4 ? p3 p4].
-         solve_cnf.
-        inv_cstep. eapply (IH n'''); eauto. omega.
-    + inv_csteps p3. simplify_elem_of. inv_cstep. }
-  intros d m p ??.
-  destruct (rtc_nsteps p) as [n pn]. inv_csteps pn.
-   destruct d5; try contradiction; simpl in *; simplify_elem_of; solve_cnf.
+     + inv_csteps p3 as [| n4 ? S4 ? p3 p4]; simpl in *.
+          left with ml2; auto. solve_cnf.
+         inv_cstep. eapply (IH n4); intuition eauto. omega.
+     + inv_csteps p3; simpl in *. right with ml2; simplify_elem_of. inv_cstep. }
+   edestruct (ax_split sr _ Haxr [CItem (sl ;; □)])
+     as [[ml2 [? [??]]] | [n' [d2 [ml2 [? [p2 ?]]]]]]; simpl in *; eauto.
+    left with ml2; auto. solve_cnf.
+   inv_csteps p2 as [| n3 ? S3 ? p2 p3]; simpl in *.
+    left with ml2; auto. solve_cnf.
+   { inv_cstep p2; try solve [simplify_stmt_elem_of].
+   * inv_csteps p3; simpl in *. now right with ml2. inv_cstep.
+   * inv_csteps p3; simpl in *. now right with ml2. inv_cstep.
+   * match goal with
+    | _ : State (Goto ?l') _ _ _ ⇨{_}^_ _ |- _ => destruct (decide (l ∈ labels sl))
+    end; simpl in *; subst.
+    + inv_csteps p3 as [| n4 ? S4 ? p3 p4]; simpl in *.
+         left with ml2; auto. solve_cnf.
+        inv_cstep. eapply (IH n4); intuition eauto. omega.
+    + inv_csteps p3; simpl in *. right with ml2; simplify_elem_of. inv_cstep. }
+  intros d ml ? p ??.
+  destruct (rtc_nsteps p) as [n pn]. inv_csteps pn; simpl in *.
+   left with ml; auto.
+   destruct d; simplify_elem_of; solve_cnf. 
   inv_cstep; eauto.
 Qed.
 
@@ -265,89 +319,100 @@ Lemma ax_if Ψ e sl sr P Q :
   Ψ ⊢ ⦃ P ∧ ∃ v, e⇓v ∧ ⌜ val_false v ⌝ ⦄ sr ⦃ Q ⦄ → 
   Ψ ⊢ ⦃ P ∧ e⇓- ⦄ IF e then sl else sr ⦃ Q ⦄.
 Proof.
-  intros Haxl Haxr A d k m d5 k5 s5 m5 p Hnf. revert d m p.
-  assert (∀ n d m,
-    (State d (CItem (IF e then □ else sr) :: k) sl m ⇨{k}^n State d5 k5 s5 m5 
+  intros Haxl Haxr d k ml mr S5 Hdisjoint p1.
+  revert d ml Hdisjoint p1.
+  assert (∀ n d ml,
+    mem_disjoint ml mr →
+    (State d (CItem (IF e then □ else sr) :: k) sl (ml ∪ mr) ⇨{k}^n S5
       ∧ down d sl
-      ∧ (A * dassert_pack Ψ (P ∧ ∃ v, e⇓v ∧ ⌜ val_true v ⌝) Q d)%A (get_stack k) m)
-    ∨ (State d (CItem (IF e then sl else □) :: k) sr m ⇨{k}^n State d5 k5 s5 m5
+      ∧ dassert_pack Ψ (P ∧ ∃ v, e⇓v ∧ ⌜ val_true v ⌝)%A Q d (get_stack k) ml)
+    ∨ (State d (CItem (IF e then sl else □) :: k) sr (ml ∪ mr) ⇨{k}^n S5
       ∧ down d sr
-      ∧ (A * dassert_pack Ψ (P ∧ ∃ v, e⇓v ∧ ⌜ val_false v ⌝) Q d)%A (get_stack k) m) →
-    k5 = k ∧ up d5 s5 ∧ (A * dassert_pack Ψ (P ∧ e⇓-) Q d5)%A (get_stack k) m5
-   ) as help.
+      ∧ dassert_pack Ψ (P ∧ ∃ v, e⇓v ∧ ⌜ val_false v ⌝)%A Q d (get_stack k) ml) →
+    ax_conclusion (dassert_pack Ψ (P ∧ e⇓-)%A Q) k mr S5) as help.
    induction n as [n IH] using lt_wf_ind.
-   intros d1 m1 [[p1 [??]] | [p1 [??]]].
-    edestruct (ax_split _ _ Haxl [CItem (IF e then □ else sr)])
-      as [n' [d2 [m2 [p2 [? [??]]]]]]; simpl in *; eauto.
-    inv_csteps p2 as [| n'' ? S3 ? p2 p3].
-     solve_cnf.
+   intros d1 ml1 ? [[p1 [??]] | [p1 [??]]].
+    edestruct (ax_split sl _ Haxl [CItem (IF e then □ else sr)])
+      as [[ml2 [? [??]]] | [n' [d2 [ml2 [? [p2 ?]]]]]]; simpl in *; eauto.
+     left with ml2; auto. solve_cnf.
+    inv_csteps p2 as [| n3 ? S3 ? p2 p3]; simpl in *.
+     left with ml2; auto. solve_cnf.
     { inv_cstep p2; try solve [simplify_stmt_elem_of].
-    * inv_csteps p3; eauto. inv_cstep.
-    * inv_csteps p3; eauto. inv_cstep.
+    * inv_csteps p3; simpl in *. now right with ml2. inv_cstep.
+    * inv_csteps p3; simpl in *. now right with ml2. inv_cstep.
     * match goal with
-      | _ : State (Goto ?l') _ _ _ ⇨{_}^_ _ |- _ => destruct (decide (l ∈ labels sr))
-      end; simpl in *; subst.
-     + inv_csteps p3 as [| n''' ? S4 ? p3 p4].
-          solve_cnf.
-         inv_cstep. eapply (IH n'''); eauto. omega.
-     + inv_csteps p3. simplify_elem_of. inv_cstep. }
-   edestruct (ax_split _ _ Haxr [CItem (IF e then sl else □)])
-     as [n' [d2 [m2 [p2 [? [??]]]]]]; simpl in *; eauto.
-   inv_csteps p2 as [| n'' ? S3 ? p2 p3].
-    solve_cnf.
-   { inv_cstep p2; try solve [simplify_stmt_elem_of].
-   * inv_csteps p3; eauto. inv_cstep.
-   * inv_csteps p3; eauto. inv_cstep.
-   * match goal with
-     | _ : State (Goto ?l') _ _ _ ⇨{_}^_ _ |- _ => destruct (decide (l ∈ labels sl))
+     | _ : State (Goto ?l') _ _ _ ⇨{_}^_ _ |- _ => destruct (decide (l ∈ labels sr))
      end; simpl in *; subst.
-    + inv_csteps p3 as [| n''' ? S4 ? p3 p4].
-         solve_cnf.
-        inv_cstep. eapply (IH n'''); eauto. omega.
-    + inv_csteps p3. simplify_elem_of. inv_cstep. }
-  intros d m p ? Hpre.
+     + inv_csteps p3 as [| n4 ? S4 ? p3 p4]; simpl in *.
+          left with ml2; auto. solve_cnf.
+         inv_cstep. eapply (IH n4); intuition eauto. omega.
+     + inv_csteps p3; simpl in *. right with ml2; simplify_elem_of. inv_cstep. }
+   edestruct (ax_split sr _ Haxr [CItem (IF e then sl else □)])
+     as [[ml2 [? [??]]] | [n' [d2 [ml2 [? [p2 ?]]]]]]; simpl in *; eauto.
+    left with ml2; auto. solve_cnf.
+   inv_csteps p2 as [| n3 ? S3 ? p2 p3]; simpl in *.
+    left with ml2; auto. solve_cnf.
+   { inv_cstep p2; try solve [simplify_stmt_elem_of].
+   * inv_csteps p3; simpl in *. now right with ml2. inv_cstep.
+   * inv_csteps p3; simpl in *. now right with ml2. inv_cstep.
+   * match goal with
+    | _ : State (Goto ?l') _ _ _ ⇨{_}^_ _ |- _ => destruct (decide (l ∈ labels sl))
+    end; simpl in *; subst.
+    + inv_csteps p3 as [| n4 ? S4 ? p3 p4]; simpl in *.
+         left with ml2; auto. solve_cnf.
+        inv_cstep. eapply (IH n4); intuition eauto. omega.
+    + inv_csteps p3; simpl in *. right with ml2; simplify_elem_of. inv_cstep. }
+  intros d ml ? p ? Hpre.
   destruct (rtc_nsteps p) as [n pn].
   destruct d; simpl in *; try contradiction.
-  * destruct Hpre as [m1 [m2 [? [? [? [? [v ?]]]]]]]; subst.
-     inv_csteps pn.
+  * destruct Hpre as [? [v ?]].
+     inv_csteps pn; simpl in *.
+      left with ml; auto.
       destruct (val_true_false_dec v); solve_cnf.
-     inv_cstep; simplify_assert_expr;
-      eapply help; [left | right]; clear help Haxl Haxr; intuition eauto; solve_assert.
-  * inv_csteps pn.
-      simplify_elem_of; solve_cnf.
+     inv_cstep; simplify_assert_expr; eapply help; eauto;
+       [left | right]; clear help Haxl Haxr; solve_assert.
+  * inv_csteps pn; simpl in *.
+      left with ml; auto. simplify_elem_of; solve_cnf.
      inv_cstep; eauto.
 Qed.
 
 Lemma ax_block_packed Ppack s :
   ax s (dassert_map (λ P, P↑* (O↦ -))%A Ppack) → ax (SBlock s) Ppack.
 Proof.
-  intros Hax A d k m d5 k5 s5 m5 p Hnf. revert d m p.
-  assert (∀ n d m b v,
-    is_free b m →
-    State d (CBlock b :: k) s (<[b:=v]>m) ⇨{k}^n State d5 k5 s5 m5 →
-    down d s →
-    (A * Ppack d)%A (get_stack k) m →
-      k5 = k ∧ up d5 s5 ∧ (A * Ppack d5)%A (get_stack k) m5
-   ).
-   intros n d1 m1 b v ? p1 ??.
-   edestruct (ax_split _ _ Hax [CBlock b] n (assert_inc_stack A))
-     as [n' [d3 [m3 [p3 [? [Hpost ?]]]]]]; simpl in *; eauto.
-    rewrite dassert_map_spec.
-    rewrite (associative assert_sep), <-assert_inc_stack_sep_distr.
-    now apply assert_alloc.
+  intros Hax d k ml mr S5 Hdisjoint p1.
+  revert d ml Hdisjoint p1.
+  assert (∀ n d ml b v,
+      mem_disjoint ml mr →
+      is_free b (ml ∪ mr) →
+      State d (CBlock b :: k) s (<[b:=v]>(ml ∪ mr)) ⇨{k}^n S5 →
+      down d s →
+      Ppack d (get_stack k) ml →
+    ax_conclusion Ppack k mr S5).
+   intros n d1 ml1 b v Hdisjoint Hfree p1 ??.
+   rewrite mem_union_insert_l in p1.
+   red in Hfree. rewrite mem_union_None_iff in Hfree. destruct Hfree.
+   assert (mem_disjoint (<[ b:=v ]>ml1) mr).
+    apply mem_disjoint_insert_l; auto.
+   clear Hdisjoint.
+   edestruct (ax_split s _ Hax [CBlock b])
+     as [[ml2 [? [??]]] | [n' [d2 [ml2 [? [p2 [? [? Hpost]]]]]]]]; simpl in *; eauto.
+     rewrite dassert_map_spec.
+     apply assert_alloc; auto.
+    left with ml2; auto. solve_cnf.
    rewrite dassert_map_spec in Hpost.
-   rewrite (associative assert_sep), <-assert_inc_stack_sep_distr in Hpost.
    apply assert_free in Hpost.
-   inv_csteps p3 as [| ???? p3 p4].
-    solve_cnf.
-   { inv_cstep p3; try solve [simplify_stmt_elem_of].
-   * inv_csteps p4. intuition. inv_cstep.
-   * inv_csteps p4. intuition. inv_cstep.
-   * inv_csteps p4. intuition. inv_cstep. }
-  intros d m p ? Hpre.
+   assert (delete b (ml2 ∪ mr) = delete b ml2 ∪ mr).
+    now rewrite mem_union_delete, (delete_lookup_None mr).
+   inv_csteps p2 as [| n3 ? S3 ? p2 p3]; simpl in *.
+    left with ml2; auto. solve_cnf.
+   { inv_cstep p2; try solve [simplify_stmt_elem_of].
+   * inv_csteps p3; simpl in *. right with (delete b ml2); auto with mem. inv_cstep.
+   * inv_csteps p3; simpl in *. right with (delete b ml2); auto with mem. inv_cstep.
+   * inv_csteps p3; simpl in *. right with (delete b ml2); auto with mem. inv_cstep. }
+  intros d ml ? p ? Hpre.
   destruct (rtc_nsteps p) as [n pn].
-  inv_csteps pn.
-   solve_cnf.
+  inv_csteps pn; simpl in *.
+   left with ml; auto. solve_cnf.
   inv_cstep; eauto.
 Qed.
 
